VisualProof/Rule/Executable/WirePrimitive.lean
@@ -1,0 +1,1 @@
+import VisualProof.Rule.Executable.WirePrimitive.Content
