VisualProof/Rule/Soundness/WirePrimitive.lean
@@ -1,0 +1,1 @@
+import VisualProof.Rule.Soundness.WirePrimitive.Content
