VisualProof/Rule/WirePrimitive.lean
@@ -1,1 +1,2 @@
 import VisualProof.Rule.WirePrimitive.Transform
+import VisualProof.Rule.WirePrimitive.Content
